A dependently-typed Term language makes everything easier

src/Denote.v
@@ -10,77 +10,28 @@ Section Denote.
 
 Context `{Env}.
 
+Import VectorNotations.
+
 (** The denotation Functor from syntactic terms over environment indices. *)
 
-Import EqNotations.
+Corollary helper {f} :
+  (let '(dom, cod) := tys[@f] in objs dom ~> objs cod)
+    -> objs (fst (tys[@f])) ~> objs (snd (tys[@f])).
+Proof. destruct (tys[@f]); auto. Defined.
+Arguments helper {f} /.
 
-Fixpoint termD_work dom (e : Term arr_idx) :
-  option (∃ cod, objs dom ~> objs cod) :=
-  match e with
-  | Ident => Some (dom; @id _ (objs dom))
-  | Morph a =>
-    match arrs a with
-    | Some (x; (y; f)) =>
-      match Eq_eq_dec x dom with
-      | Specif.left edom =>
-        Some (y; rew [fun x => objs x ~> objs y] edom in f)
-      | _ => None
-      end
-    | _ => None
-    end
-  | Comp f g =>
-    match termD_work dom g with
-    | Some (mid; g) =>
-      match termD_work mid f with
-      | Some (y; f) => Some (y; f ∘ g)
-      | _ => None
-      end
-    | _ => None
-    end
+Fixpoint termD {dom cod} (t : Term tys dom cod) : objs dom ~> objs cod :=
+  match t with
+  | Ident => id
+  | Morph f => helper (ith arrs f)
+  | Comp f g => termD f ∘ termD g
   end.
 
-Definition termD dom cod (e : Term arr_idx) : option (objs dom ~> objs cod) :=
-  match termD_work dom e with
-  | Some (y; f) =>
-    match Eq_eq_dec y cod with
-    | Specif.left ecod => Some (rew [fun y => objs dom ~> objs y] ecod in f)
-    | _ => None
-    end
-  | _ => None
-  end.
-
-Lemma termD_app {dom cod f g} :
-  ∃ mid, termD dom cod (Comp f g)
-           = termD mid cod f ∘[opt_arrs] termD dom mid g.
-Proof.
-  unfold termD; simpl.
-  destruct (termD_work dom g) eqn:?.
-  - destruct s.
-    exists x.
-    destruct f; simpl; intros.
-    + rewrite Pos_eq_dec_refl.
-      destruct (Pos.eq_dec x cod); subst; auto.
-    + destruct (arrs a) eqn:?.
-        destruct s, s.
-        repeat desg; repeat desh; cat.
-      repeat desg; repeat desh; cat.
-    + destruct (termD_work x f2) eqn:?; auto.
-      destruct s.
-      destruct (termD_work x0 f1) eqn:?; auto.
-      destruct s.
-      rewrite Pos_eq_dec_refl.
-      destruct (Pos.eq_dec x1 cod); subst; auto.
-  - exists cod.
-    destruct (termD_work cod f) eqn:?; auto.
-    destruct s.
-    destruct (Pos.eq_dec x cod); subst; auto.
-Qed.
-
-Fixpoint exprD (e : Expr arr_idx) : Type :=
+Fixpoint exprD (e : Expr) : Type :=
   match e with
   | Top           => True
   | Bottom        => False
-  | Equiv x y f g => termD x y f ≈ termD x y g
+  | Equiv _ _ f g => termD f ≈ termD g
   | And p q       => exprD p ∧ exprD q
   | Or p q        => exprD p + exprD q
   | Impl p q      => exprD p -> exprD q
