src/Expr.v
@@ -7,38 +7,42 @@ Unset Equations WithK.
 
 Generalizable All Variables.
 
-Inductive Term {A : Type} : Type :=
-  | Ident : Term
-  | Morph (a : A) : Term
-  | Comp (f : Term) (g : Term) : Term.
+Import VectorNotations.
 
-Arguments Term : clear implicits.
+Inductive Term {a} (tys : Vector.t (obj_idx * obj_idx) a) :
+  obj_idx -> obj_idx -> Type :=
+  | Ident : ∀ dom, Term tys dom dom
+  | Morph (f : arr_idx a) : Term tys (fst (tys[@f])) (snd (tys[@f]))
+  | Comp (dom mid cod : obj_idx)
+         (f : Term tys mid cod) (g : Term tys dom mid) :
+      Term tys dom cod.
 
-Fixpoint term_size `(t : Term A) : nat :=
+Arguments Ident {a tys dom}.
+Arguments Morph {a tys} f.
+Arguments Comp {a tys dom mid cod} f g.
+
+Derive Signature NoConfusion Subterm for Term.
+
+Section Expr.
+
+Context `{Env}.
+
+Fixpoint term_size `(t : Term tys d c) : nat :=
   match t with
   | Ident    => 1%nat
   | Morph _  => 1%nat
   | Comp f g => 1%nat + term_size f + term_size g
   end.
 
-Fixpoint term_map {A B : Type} (f : A -> B) (t : Term A) : Term B :=
-  match t with
-  | Ident    => Ident
-  | Morph a  => Morph (f a)
-  | Comp l r => Comp (term_map f l) (term_map f r)
-  end.
-
-Inductive Expr {A : Type} : Type :=
+Inductive Expr : Type :=
   | Top
   | Bottom
-  | Equiv (x y : obj_idx) (f g : Term A)
+  | Equiv (d c : obj_idx) (f g : Term tys d c)
   | And   (p q : Expr)
   | Or    (p q : Expr)
   | Impl  (p q : Expr).
 
-Arguments Expr : clear implicits.
-
-Fixpoint expr_size `(t : Expr A) : nat :=
+Fixpoint expr_size (t : Expr) : nat :=
   match t with
   | Top           => 1%nat
   | Bottom        => 1%nat
@@ -48,130 +52,7 @@ Fixpoint expr_size `(t : Expr A) : nat :=
   | Impl p q      => 1%nat + expr_size p + expr_size q
   end.
 
-Remark all_exprs_have_size {A} e : (0 < expr_size (A:=A) e)%nat.
+Remark all_exprs_have_size e : (0 < expr_size e)%nat.
 Proof. induction e; simpl; omega. Qed.
 
-(** Syntactic terms are endofunctors on Coq. *)
-
-Program Definition TermF : Coq ⟶ Coq := {|
-  fmap := @term_map
-|}.
-Next Obligation.
-  proper.
-  induction x1; simpl; auto.
-    now rewrite H.
-  now rewrite IHx1_1, IHx1_2.
-Qed.
-Next Obligation.
-  induction x0; simpl; auto.
-  now rewrite IHx0_1, IHx0_2.
-Qed.
-Next Obligation.
-  induction x0; simpl; auto.
-  now rewrite IHx0_1, IHx0_2.
-Qed.
-
-Global Program Instance TermF_Map : EndoFunctor TermF :=
-  Functor_EndoFunctor (F:=TermF).
-
-(** A lawful way of saying that Term is Foldable. *)
-
-Fixpoint arrows {a} (t : Term a) : list a :=
-  match t with
-  | Ident    => nil
-  | Morph a  => [a]
-  | Comp f g => arrows f ++ arrows g
-  end.
-
-Definition unarrows `(fs : list A) : Term A :=
-  List.fold_right (fun f rest => Comp (Morph f) rest) Ident fs.
-
-Lemma unarrows_arrows `(f : list A) : arrows (unarrows f) = f.
-Proof. induction f; simpl; auto; now f_equal. Qed.
-
-Global Program Instance Term_Foldable : TermF ⟹ listF := {
-  transform := fun _ => arrows
-}.
-Next Obligation.
-  induction x0; simpl; auto.
-  rewrite <- IHx0_1, <- IHx0_2.
-  now rewrite List.map_app.
-Qed.
-Next Obligation.
-  induction x0; simpl; auto.
-  rewrite IHx0_1, IHx0_2.
-  now rewrite List.map_app.
-Qed.
-
-(** Term is also Traversable.
-
-    jww (2018-03-10): For the moment this is too painful to do this generally,
-    so we do it for the few cases that we need. *)
-
-Fixpoint Term_option_sequence {a} (x : Term (option a)) : option (Term a) :=
-  match x with
-  | Ident => Some Ident
-  | Morph a => map[optionF] Morph a
-  | Comp f g =>
-    match Term_option_sequence f with
-    | None => None
-    | Some f' =>
-      match Term_option_sequence g with
-      | None => None
-      | Some g' =>
-        Some (Comp f' g')
-      end
-    end
-  end.
-
-Global Program Instance Term_option_Traversable :
-  TermF ○ optionF ⟹ optionF ○ TermF := {
-  transform := fun _ => Term_option_sequence
-}.
-Next Obligation.
-  intros.
-  induction x0; simpl; auto.
-  - destruct a; auto.
-  - rewrite <- IHx0_1, <- IHx0_2.
-    clear IHx0_1 IHx0_2.
-    do 2 destruct (Term_option_sequence _); auto.
-Qed.
-Next Obligation.
-  induction x0; simpl; auto.
-  - destruct a; auto.
-  - rewrite IHx0_1, IHx0_2.
-    clear IHx0_1 IHx0_2.
-    do 2 destruct (Term_option_sequence _); auto.
-Qed.
-
-(** The category of syntactic terms, equivalent up to normalization. *)
-
-Definition Term_equiv `{Setoid A} (f g : Term A) : Type :=
-  arrows f = arrows g.
-Arguments Term_equiv {A _} f g /.
-
-Program Instance Term_equivalence `{Setoid A} :
-  Equivalence Term_equiv.
-
-Instance Term_Setoid `{Setoid A} : Setoid (Term A) := {|
-  equiv := Term_equiv;
-  setoid_equiv := Term_equivalence
-|}.
-
-Program Instance Comp_Proper `{Setoid A} :
-  Proper (equiv ==> equiv ==> equiv) (@Comp A).
-Next Obligation.
-  proper.
-  simpl in *.
-  now rewrite X, X0.
-Qed.
-
-Program Instance Terms (A : Type) `{Setoid A} : Category := {|
-  obj := obj_idx;
-  hom := fun _ _ => Term A;
-  id := fun _ => Ident;
-  compose := fun _ _ _ => Comp
-|}.
-Next Obligation. now rewrite List.app_nil_r. Defined.
-Next Obligation. now rewrite List.app_assoc. Defined.
-Next Obligation. now rewrite List.app_assoc. Defined.
+End Expr.
