src/IList.v
@@ -1,0 +1,150 @@
+Require Import Coq.Vectors.Vector.
+
+Generalizable All Variables.
+
+Section ilist.
+
+Import VectorNotations.
+
+Open Scope vector_scope.
+Open Scope nat_scope.
+
+Definition Vector_caseS'
+           {A'} (Q : nat -> Type)
+           (P : forall {n} (v : Vector.t A' (S n)), Q n -> Type)
+           (H : forall h {n} t q, @P n (h :: t) q) {n} (v: Vector.t A' (S n))
+           (q : Q n)
+: P v q.
+Proof.
+  specialize (fun h t => H h _ t q).
+  change n with (pred (S n)) in H, q |- *.
+  set (Sn := S n) in *.
+  pose (fun Sn (v : Vector.t A' Sn) (q : Q (pred Sn)) =>
+          match Sn return Vector.t A' Sn -> Q (pred Sn) -> Type with
+            | S n' => P n'
+            | 0 => fun _ _ => True
+          end v q) as P'.
+  change (match Sn return Type with
+            | 0 => True
+            | _ => P' Sn v q
+          end).
+  change (forall h (t : match Sn with
+                          | S n' => Vector.t A' n'
+                          | 0 => Vector.t A' Sn
+                        end),
+            P' Sn (match Sn return match Sn with
+                                     | S n' => Vector.t A' n'
+                                     | 0 => Vector.t A' Sn
+                                   end -> Vector.t A' Sn
+                   with
+                     | S _ => fun t => h :: t
+                     | 0 => fun t => t
+                   end t) q) in H.
+  clearbody P'; clear P.
+  clearbody Sn.
+  destruct v as [|h ? t].
+  { constructor. }
+  { apply H. }
+Defined.
+
+Context {A : Type}. (* The indexing type. *)
+Context {B : A -> Type}. (* The type of indexed elements. *)
+
+Record prim_prod A B : Type :=
+  { prim_fst : A;
+    prim_snd : B }.
+
+Arguments prim_fst {A B} _.
+Arguments prim_snd {A B} _.
+
+Fixpoint ilist {n} (l : Vector.t A n) : Type :=
+  match l with
+    | [] => unit
+    | a :: l => @prim_prod (B a) (ilist l)
+  end.
+
+Definition vec_of `(x : @ilist n l) := l.
+
+Definition icons
+           (a : A)
+           {n}
+           {l : Vector.t A n}
+           (b : B a)
+           (il : ilist l)
+: ilist (a :: l)
+  := {| prim_fst := b; prim_snd := il |}.
+
+Definition inil : ilist [] := tt.
+
+(* Get the car of an ilist. *)
+Definition ilist_hd {n} {As : Vector.t A n} (il : ilist As) :
+  match As return ilist As -> Type with
+    | a :: As' => fun il => B a
+    | [] => fun _ => unit
+  end il :=
+  match As return
+        forall (il : ilist As),
+          match As return ilist As -> Type with
+            | a :: As' => fun il => B a
+            | [] => fun _ => unit
+          end il with
+    | a :: As => fun il => prim_fst il
+    | [] => fun il => tt
+  end il.
+
+(* Get the cdr of an ilist. *)
+Definition ilist_tl {n} {As : Vector.t A n} (il : ilist As) :
+  match As return ilist As -> Type with
+    | a :: As' => fun il => ilist As'
+    | [] => fun _ => unit
+  end il :=
+  match As return
+        forall (il : ilist As),
+          match As return ilist As -> Type with
+            | a :: As' => fun il => ilist As'
+            | [] => fun _ => unit
+          end il with
+    | a :: As => fun il => prim_snd il
+    | [] => fun il => tt
+  end il.
+
+Fixpoint ith
+           {m : nat}
+           {As : Vector.t A m}
+           (il : ilist As)
+           (n : Fin.t m)
+: B (Vector.nth As n) :=
+  match n in Fin.t m return
+        forall (As : Vector.t A m),
+          ilist As
+          -> B (Vector.nth As n) with
+    | @Fin.F1 k =>
+      fun As =>
+        Vector.caseS (fun n As => ilist As
+                                  -> B (Vector.nth As (@Fin.F1 n)))
+                     (fun h n t => ilist_hd) As
+    | @Fin.FS k n' =>
+      fun As =>
+        Vector_caseS' Fin.t
+                      (fun n As n' => ilist As
+                                      -> B (Vector.nth As (@Fin.FS n n')))
+                      (fun h n t m il => ith (ilist_tl il) m)
+                      As n'
+  end As il.
+
+Infix "++" := Vector.append.
+
+Fixpoint ilist_app {n} {As : Vector.t A n}
+  : forall {n'} {As' : Vector.t A n'},  ilist As -> ilist As' -> ilist (As ++ As') :=
+    match As return
+          forall {n'} (As' : Vector.t A n'),
+            ilist As -> ilist As' -> ilist (As ++ As') with
+      | [] =>
+        fun n' As' il il' => il'
+      | a :: As'' =>
+        fun n' As' il il' =>
+          {| prim_fst := ilist_hd il;
+             prim_snd := ilist_app (ilist_tl il) il' |}
+    end.
+
+End ilist.
